src/trans/SimGlobal.v
@@ -1,0 +1,49 @@
+Require Import RelationClasses.
+
+From sflib Require Import sflib.
+From Paco Require Import paco.
+
+From PromisingLib Require Import Axioms.
+From PromisingLib Require Import Basic.
+From PromisingLib Require Import Loc.
+From PromisingLib Require Import DenseOrder.
+From PromisingLib Require Import Language.
+From PromisingLib Require Import Event.
+
+Require Import Time.
+Require Import View.
+Require Import BoolMap.
+Require Import Promises.
+Require Import Reserves.
+Require Import Cell.
+Require Import Memory.
+Require Import Global.
+Require Import TView.
+Require Import Local.
+Require Import Thread.
+Require Import Configuration.
+
+Require Import SimMemory.
+
+Set Implicit Arguments.
+
+
+Variant sim_global (gl_src gl_tgt: Global.t): Prop :=
+| sim_global_intro
+    (SC: TimeMap.le (Global.sc gl_src) (Global.sc gl_tgt))
+    (PROMISES: Global.promises gl_src = Global.promises gl_tgt)
+    (RESERVES: Global.reserves gl_src = Global.reserves gl_tgt)
+    (MEMORY: sim_memory (Global.memory gl_src) (Global.memory gl_tgt))
+.
+#[export] Hint Constructors sim_global: core.
+
+Global Program Instance sim_global_PreOrder: PreOrder sim_global.
+Next Obligation.
+  ii. destruct x. econs; refl.
+Qed.
+Next Obligation.
+  ii. destruct x, y, z. inv H. inv H0. ss. subst.
+  econs; ss; etrans; eauto.
+Qed.
+
+
