src/trans/SimLocal.v
@@ -1,0 +1,53 @@
+Require Import RelationClasses.
+
+From sflib Require Import sflib.
+From Paco Require Import paco.
+
+From PromisingLib Require Import Axioms.
+From PromisingLib Require Import Basic.
+From PromisingLib Require Import Loc.
+From PromisingLib Require Import DenseOrder.
+From PromisingLib Require Import Language.
+From PromisingLib Require Import Event.
+
+Require Import Time.
+Require Import View.
+Require Import BoolMap.
+Require Import Promises.
+Require Import Reserves.
+Require Import Cell.
+Require Import Memory.
+Require Import Global.
+Require Import TView.
+Require Import Local.
+Require Import Thread.
+Require Import Configuration.
+
+Set Implicit Arguments.
+
+
+Variant sim_local (lc_src lc_tgt: Local.t): Prop :=
+| sim_local_intro
+    (TVIEW: TView.le (Local.tview lc_src) (Local.tview lc_tgt))
+    (PROMISES: Local.promises lc_src = Local.promises lc_tgt)
+    (RESERVES: Local.reserves lc_src = Local.reserves lc_tgt)
+.
+#[export] Hint Constructors sim_local: core.
+
+Global Program Instance sim_local_PreOrder: PreOrder sim_local.
+Next Obligation.
+  ii. destruct x. econs; refl.
+Qed.
+Next Obligation.
+  ii. destruct x, y, z. inv H. inv H0. ss. subst.
+  econs; ss. etrans; eauto.
+Qed.
+
+Lemma sim_local_is_terminal
+      lc_src lc_tgt
+      (SIM: sim_local lc_src lc_tgt):
+  Local.is_terminal lc_src <-> Local.is_terminal lc_tgt.
+Proof.
+  destruct lc_src, lc_tgt. inv SIM. ss.
+  split; i; inv H; ss.
+Qed.
